% --------------------------------------------------------------
% This is all preamble stuff that you don't have to worry about.
% Head down to where it says "Start here"
% --------------------------------------------------------------

\documentclass[12pt]{article}

\usepackage[margin=1in]{geometry} 
\usepackage{amsmath,amsthm,amssymb}
\usepackage{color}

\makeatletter

\renewcommand\section{\@startsection {section}{1}{\z@}%
	{-3.5ex \@plus -1ex \@minus -.2ex}%
	{2.3ex \@plus.2ex}%
	{\normalfont\large\bfseries}}% from \Large
\renewcommand\subsection{\@startsection{subsection}{2}{\z@}%
	{-3.25ex\@plus -1ex \@minus -.2ex}%
	{1.5ex \@plus .2ex}%
	{\normalfont\large\bfseries}}% from \large
\makeatother

\begin{document}
	
	% --------------------------------------------------------------
	%                         Start here
	% --------------------------------------------------------------
	
	%\renewcommand{\qedsymbol}{\filledbox}
	
	\title{\textbf{Machine Learning Assignment \#2}\\
	Universit{\"a}t Bern}%replace X with the appropriate number
	\author{Lin Bai 09935404} %replace with your name
	
	\maketitle
	
	%%%%%%%%%%%%%%%%%%%%%%%%%%%%%%%%%%%%%%%%%%%%%%%%%%%%%%%%%%%%%%%%%%%%%%%%%%%%%%%%%%%%%%%%
	%%%%%%   notations
	%%%%%%%%%%%%%%%%%%%%%%%%%%%%%%%%%%%%%%%%%%%%%%%%%%%%%%%%%%%%%%%%%%%%%%%%%%%%%%%%%%%%%%%%
	\section*{Notations}
	$A, B, C\in \mathbb{R}^{n\times n}$ are $n\times n$ matrices, $x, a, b\in \mathbb{R}^n$ are column vectors.

	%%%%%%%%%%%%%%%%%%%%%%%%%%%%%%%%%%%%%%%%%%%%%%%%%%%%%%%%%%%%%%%%%%%%%%%%%%%%%%%%%%%%%%%%
	%%%%%%   question 1, sub question (a)
	%%%%%%%%%%%%%%%%%%%%%%%%%%%%%%%%%%%%%%%%%%%%%%%%%%%%%%%%%%%%%%%%%%%%%%%%%%%%%%%%%%%%%%%%
	\section*{Solution of question 1}
	\subsection*{(a)}
	Since both $a$ and $x$ are column vector with n elements.\\
	we know $a^{T}x = (a_1, a_2, ... a_n)$
	\begin{equation}\label{a_time_x}
	a^{T}x=  
	\left(  
	\begin{array}{cccc}  
	a_{1}, &  
	a_{2}, &   
	\cdots &  
	a_{n}  
	\end{array}  
	\right)  
	\left(  
	\begin{array}{c}  
	x_{1} \\   
	x_{2} \\  
	\vdots \\  
	x_{n}  
	\end{array}  
	\right)
	=a_1x_1+a_2x_2+\cdots a_nx_n
	= \sum_{i=1}^n a_i x_i
	\end{equation}
	according to the mathematics definition of $\nabla_xf(x)$ and equation (\ref{a_time_x}), we know
	\begin{equation}\label{gradient_atx}
	\nabla_x(a^Tx)=
	\left(  
	\begin{array}{c}  
	\frac{\partial(a^Tx)}{\partial x_1} \\
	\frac{\partial(a^Tx)}{\partial x_2} \\
	\vdots \\
	\frac{\partial(a^Tx)}{\partial x_n} 
	\end{array}
	\right)
	=
	\left(  
	\begin{array}{c}  
	\frac{\partial(\sum_{i=1}^n a_i x_i)}{\partial x_1} \\
	\frac{\partial(\sum_{i=1}^n a_i x_i)}{\partial x_2} \\
	\vdots \\
	\frac{\partial(\sum_{i=1}^n a_i x_i)}{\partial x_n} 
	\end{array}
	\right)
	\end{equation}
	due to
	\begin{equation}\label{gradient_atx_i}
	\frac{\partial(\sum_{i=1}^n a_i x_i)}{\partial x_i}=a_i
	\end{equation}
	we know the equation (\ref{gradient_atx}) will become
	\begin{equation}\label{gradient_atx_final}
	\nabla_x(a^Tx)=
	\left(  
	\begin{array}{c}  
	a_1 \\
	a_2 \\
	\vdots \\
	a_n 
	\end{array}
	\right)
	= a
	\end{equation}
	therefore, $$\nabla_x(a^Tx)=a$$
	
	%%%%%%%%%%%%%%%%%%%%%%%%%%%%%%%%%%%%%%%%%%%%%%%%%%%%%%%%%%%%%%%%%%%%%%%%%%%%%%%%%%%%%%%%
	%%%%%%%   question 1, sub question (b)
	%%%%%%%%%%%%%%%%%%%%%%%%%%%%%%%%%%%%%%%%%%%%%%%%%%%%%%%%%%%%%%%%%%%%%%%%%%%%%%%%%%%%%%%%
	\subsection*{(b)}
	The product of $x^TA$ is
	\begin{equation}\label{xt_a}
	\begin{split}
	x^TA=
	\left( 
	\begin{array}{cccc}  
	x_1 &
	x_2 &
	\cdots &
	x_n 
	\end{array}
	\right)
	\left(  
	\begin{array}{c}  
	a_{11}, a_{12},\cdots a_{1n} \\
	a_{21}, a_{22},\cdots a_{2n} \\
	\cdots \\
	a_{n1}, a_{n2},\cdots a_{nn} \\
	\end{array}  
	\right)\\
	=
	\left( 
	\begin{array}{cccc} 
	\sum_{p=1}^n x_pa_{p1}, & \sum_{p=1}^n x_pa_{p2}, & \cdots & \sum_{p=1}^n x_pa_{pn} 
	\end{array}  
	\right)\\
	\end{split}
	\end{equation}
	same principle, $x^TAx$'s product is
	\begin{equation}\label{xt_a_x}
	x^TAx = (\sum_{p=1}^n x_pa_{p1})x_1 + (\sum_{p=1}^n x_pa_{p2})x_2 + \cdots (\sum_{p=1}^n x_pa_{pn})x_n
	= \sum_{p=1}^n \sum_{q=1}^n x_pa_{pq}x_q
	\end{equation}
	therefore the gradient of $x^TAx$ is
	\begin{equation}\label{gradient_xtax}
	\nabla_x(x^TAx)=
	\left(  
	\begin{array}{c}  
	\frac{\partial(\sum_{p=1}^n \sum_{q=1}^n x_pa_{pq}x_q)}{\partial x_1} \\
	\frac{\partial(\sum_{p=1}^n \sum_{q=1}^n x_pa_{pq}x_q)}{\partial x_2} \\
	\vdots \\
	\frac{\partial(\sum_{p=1}^n \sum_{q=1}^n x_pa_{pq}x_qs)}{\partial x_n} 
	\end{array}
	\right)
	\end{equation}
	take question (\ref{gradient_xtax})'s $i$th element for example, the $\frac{\partial(\sum_{p=1}^n \sum_{q=1}^n x_pa_{pq}x_q)}{\partial x_i}$ contains one 2-order expression of $x_i$, that is ${x_i}^2a_{ii}$; and two 1-order expressions, they are $\sum_{p} x_pa_{pi}$ and $\sum_{q} x_qa_{iq}$, where $q, p \in [1, n]$ and $p\neq q\neq i$.
	\begin{equation}\label{gradient_xtax_i}
	\frac{\partial(\sum_{p=1}^n \sum_{q=1}^n x_pa_{pq}x_q)}{\partial x_i} \\
	=\frac{\partial(\sum_{p} x_ix_pa_{pi}+\sum_{q} x_ix_qa_{iq}+x_ix_ia_{ii})}{\partial x_i}
	\end{equation}
	, where $q, p \in [1, n]$ and $p\neq q\neq i$.
	\\
	since matrix $A$ is symmetrical, $a_{ij}=a_{ji}$, equation (\ref{gradient_xtax_i}) becomes
	\begin{equation}\label{gradient_xtax_i_mod}
	\frac{\partial(\sum_{p} x_ix_pa_{pi}+\sum_{q} x_ix_qa_{iq}+x_ix_ia_{ii})}{\partial x_i}
	=\frac{\partial(2\sum_{p} x_ix_pa_{pi}+x_i^2a_{ii})}{\partial x_i}
	=2\sum_{p} x_pa_{pi}+2x_ia_{ii}
	\end{equation}
	, where $p \in [1, n]$ and $p\neq i$.\\
	Since $2x_ia_{ii}$ is the expression of $x_ix_pa_{pi}$ when $p=i$, we can get
	\begin{equation}\label{gradient_xtax_i_final}
	2\sum_{p} x_ix_pa_{pi}+2x_ia_{ii}
	=2\sum_{k=1}^n x_ka_{ik}
	\end{equation}
	, where $p \in [1, n]$ and $p\neq i$.\\
	So, the $i$th element of $\nabla_x(x^TAx)$ is $2\sum_{k=1}^n x_ka_{ik}$.\\
	\\
	\noindent
	On the other hand, the $i$th element of $2Ax$ is $2\sum_{k=1}^n a_{ik}x_k$ as well.Therefore, $\nabla_x(x^TAx)=2Ax$ is proved.
	
	%%%%%%%%%%%%%%%%%%%%%%%%%%%%%%%%%%%%%%%%%%%%%%%%%%%%%%%%%%%%%%%%%%%%%%%%%%%%%%%%%%%%%%%%
	%%%%%%   question 2
	%%%%%%%%%%%%%%%%%%%%%%%%%%%%%%%%%%%%%%%%%%%%%%%%%%%%%%%%%%%%%%%%%%%%%%%%%%%%%%%%%%%%%%%%
	\section*{Solution of question 2}
	
	\begin{equation}\label{Ax-b_grad_1}
	\begin{split}
	\nabla_x\lVert Ax-b\rVert_2^2
	=\nabla_x (Ax-b)^T(Ax-b)
	=\nabla_x (x^TA^TAx-2b^TAx+b^Tb) \\
	=\nabla_x x^TA^TAx-\nabla_x2b^TAx+\nabla_x b^Tb
	\end{split}
	\end{equation}
	According to the result of question 1 $\nabla_x(x^TAx)=2Ax$, we know,
	\begin{equation}\label{Ax-b_grad_2}
	\nabla_x\lVert Ax-b\rVert_2^2
	=\nabla_x x^TA^TAx-\nabla_x2b^TAx+\nabla_x b^Tb
	=2A^TAx-2A^Tb
	\end{equation}
	
	%%%%%%%%%%%%%%%%%%%%%%%%%%%%%%%%%%%%%%%%%%%%%%%%%%%%%%%%%%%%%%%%%%%%%%%%%%%%%%%%%%%%%%%%
	%%%%%%   question 3, sub question (a)
	%%%%%%%%%%%%%%%%%%%%%%%%%%%%%%%%%%%%%%%%%%%%%%%%%%%%%%%%%%%%%%%%%%%%%%%%%%%%%%%%%%%%%%%%
	\section*{Solution of question 3}
	\subsection*{(a)}
	the trace of matrix $A$ is $\sum_{i=1}^n a_{ii}$.\\
	so the gradient is $tr(A)$ is
	\begin{equation}\label{trA_grad}
	\nabla_A(tr(A))=
	\left(  
	\begin{array}{cccc}  
	\frac{\partial\sum_{i=1}^n a_{ii}}{\partial a_{11}} & \frac{\partial\sum_{i=1}^n a_{ii}}{\partial a_{12}} \cdots \frac{\partial\sum_{i=1}^n a_{ii}}{\partial a_{1n}}\\
	\frac{\partial\sum_{i=1}^n a_{ii}}{\partial a_{21}} & \frac{\partial\sum_{i=1}^n a_{ii}}{\partial a_{22}} \cdots \frac{\partial\sum_{i=1}^n a_{ii}}{\partial a_{1n}}\\
	\vdots \\
	\frac{\partial\sum_{i=1}^n a_{ii}}{\partial a_{n1}} & \frac{\partial\sum_{i=1}^n a_{ii}}{\partial a_{n2}} \cdots \frac{\partial\sum_{i=1}^n a_{ii}}{\partial a_{nn}}\\
	\end{array}
	\right)
	=
	\left(  
	\begin{array}{cccc}
	1 & 0 & \cdots & 0\\
	0 & 1 & \cdots & 0\\
	\vdots\\
	0 & 0 & \cdots & 1\\
	\end{array}
	\right)
	= I
	\end{equation}
	
	%%%%%%%%%%%%%%%%%%%%%%%%%%%%%%%%%%%%%%%%%%%%%%%%%%%%%%%%%%%%%%%%%%%%%%%%%%%%%%%%%%%%%%%%
	%%%%%%   question 3, sub question (b)
	%%%%%%%%%%%%%%%%%%%%%%%%%%%%%%%%%%%%%%%%%%%%%%%%%%%%%%%%%%%%%%%%%%%%%%%%%%%%%%%%%%%%%%%%
	\subsection*{(b)}
	The trace of product $AB$ is
	\begin{equation}\label{ab_ii}
	tr(AB)=\sum_{i=1}^n (AB)_{(i,i)}=\sum_{i=1}^n\sum_{j=1}^n a_{ij}b_{ji}
	\end{equation}
	so the gradient of $AB$ respect to $A$ is
	\begin{equation}\label{trAB_grad}
	\begin{split}
	\nabla_A(tr(AB))=&
	\left(  
	\begin{array}{cccc}
	\frac{\partial\sum_{i=1}^n\sum_{j=1}^n a_{ij}b_{ji}}{\partial a_{11}} & \frac{\partial\sum_{i=1}^n\sum_{j=1}^n a_{ij}b_{ji}}{\partial a_{12}} \cdots \frac{\partial\sum_{i=1}^n\sum_{j=1}^n a_{ij}b_{ji}}{\partial a_{1n}}\\
	\frac{\partial\sum_{i=1}^n\sum_{j=1}^n a_{ij}b_{ji}}{\partial a_{21}} & \frac{\partial\sum_{i=1}^n\sum_{j=1}^n a_{ij}b_{ji}}{\partial a_{22}} \cdots \frac{\partial\sum_{i=1}^n\sum_{j=1}^n a_{ij}b_{ji}}{\partial a_{1n}}\\
	\vdots \\
	\frac{\partial\sum_{i=1}^n\sum_{j=1}^n a_{ij}b_{ji}}{\partial a_{n1}} & \frac{\partial\sum_{i=1}^n\sum_{j=1}^n a_{ij}b_{ji}}{\partial a_{n2}} \cdots \frac{\partial\sum_{i=1}^n\sum_{j=1}^n a_{ij}b_{ji}}{\partial a_{nn}}\\	
	\end{array}
	\right)\\
	&=
	\left(
	\begin{array}{cccc}	
	b_{11} & b_{21} & \cdots & b_{n1}\\
	b_{12} & b_{22} & \cdots & b_{n2}\\
	\vdots \\
	b_{1n} & b_{2n} & \cdots & b_{nn}\\
	\end{array}
	\right)
	=B^T
	\end{split}
	\end{equation}
	
	%%%%%%%%%%%%%%%%%%%%%%%%%%%%%%%%%%%%%%%%%%%%%%%%%%%%%%%%%%%%%%%%%%%%%%%%%%%%%%%%%%%%%%%%
	%%%%%%   question 3, sub question (c)
	%%%%%%%%%%%%%%%%%%%%%%%%%%%%%%%%%%%%%%%%%%%%%%%%%%%%%%%%%%%%%%%%%%%%%%%%%%%%%%%%%%%%%%%%
	\subsection*{(c)}
	from the conclusion from (b), we know
	\begin{equation}\label{aa_ii}
	tr(A^TA)=\sum_{i=1}^n (A^TA)_{(i,i)}=\sum_{i=1}^n\sum_{j=1}^n a_{ij}^2
	\end{equation}
	so the gradient of $A^TA$ respect to $A$ is
	\begin{equation}\label{trAA_grad}
	\begin{split}
	\nabla_A(tr(A^TA))=&
	\left(  
	\begin{array}{cccc}
	\frac{\partial\sum_{i=1}^n\sum_{j=1}^n a_{ij}^2}{\partial a_{11}} & \frac{\partial\sum_{i=1}^n\sum_{j=1}^n a_{ij}^2}{\partial a_{12}} \cdots \frac{\partial\sum_{i=1}^n\sum_{j=1}^n a_{ij}^2}{\partial a_{1n}}\\
	\frac{\partial\sum_{i=1}^n\sum_{j=1}^n a_{ij}^2}{\partial a_{21}} & \frac{\partial\sum_{i=1}^n\sum_{j=1}^n a_{ij}^2}{\partial a_{22}} \cdots \frac{\partial\sum_{i=1}^n\sum_{j=1}^n a_{ij}^2}{\partial a_{2n}}\\
	\vdots \\
	\frac{\partial\sum_{i=1}^n\sum_{j=1}^n a_{ij}^2}{\partial a_{n1}} & \frac{\partial\sum_{i=1}^n\sum_{j=1}^n a_{ij}^2}{\partial a_{n2}} \cdots \frac{\partial\sum_{i=1}^n\sum_{j=1}^n a_{ij}^2}{\partial a_{nn}}\\	
	\end{array}
	\right)\\
	&=
	\left(  
	\begin{array}{cccc}
	\frac{\partial a_{11}^2}{\partial a_{11}} & \frac{\partial a_{12}^2}{\partial a_{12}} \cdots \frac{\partial a_{1n}^2}{\partial a_{1n}}\\
	\frac{\partial a_{21}^2}{\partial a_{21}} & \frac{\partial a_{22}^2}{\partial a_{22}} \cdots \frac{\partial a_{2n}^2}{\partial a_{2n}}\\
	\vdots \\
	\frac{\partial a_{n1}^2}{\partial a_{n1}} & \frac{\partial a_{n2}^2}{\partial a_{n2}} \cdots \frac{\partial a_{nn}^2}{\partial a_{nn}}\\	
	\end{array}
	\right)\\
	&=
	\left(
	\begin{array}{cccc}	
	2a_{11} & 2a_{12} & \cdots & 2a_{1n}\\
	2a_{21} & 2a_{22} & \cdots & 2a_{2n}\\
	\vdots \\
	2a_{n1} & 2a_{n2} & \cdots & 2a_{nn}\\
	\end{array}
	\right)
	=2A
	\end{split}
	\end{equation}
	
	%%%%%%%%%%%%%%%%%%%%%%%%%%%%%%%%%%%%%%%%%%%%%%%%%%%%%%%%%%%%%%%%%%%%%%%%%%%%%%%%%%%%%%%%
	%%%%%%   question 4, sub question (a)
	%%%%%%%%%%%%%%%%%%%%%%%%%%%%%%%%%%%%%%%%%%%%%%%%%%%%%%%%%%%%%%%%%%%%%%%%%%%%%%%%%%%%%%%%
	\subsection*{Solution of question 4}
	\subsection*{(a)}
	the 4 matrix norm properties are:
	\begin{enumerate}
		\item For all $x\in \mathbb{R}^{n}$, $f(x)\geq0$ (non-negativity)
		\item $f(x)=0$ if and only if $x=0$ (definiteness)
		\item For all $x\in \mathbb{R}^{n}$, $t\in \mathbb{R}$, $f(tx)=\mid t\mid f(x)$ (homogeneity)
		\item For all $x, y\in \mathbb{R}^{n}$, $f(x+y)\le f(x)+f(y)$ (triangle inequality)
	\end{enumerate}
	The definition of Frobenius norm is
	\begin{equation}
	\lVert A\rVert_F=\sqrt{\sum_{i=1}^n\sum_{j=1}^na_{ij}^2}=\sqrt{tr(A^TA)}
	\end{equation}
	\textbf{non-negativity}\\
	since matrix is in real number space, $A_{ij}^2\geq 0$, so sum of each $A_{ij}^2$ must be greater or equal to 0, so as it's square root. So $\lVert A\rVert_F\geq 0$\\
	\textbf{definiteness}\\
	if $\sqrt{\sum_{i=1}^m\sum_{j=1}^nA_{ij}^2}=0$, any single $A_{ij}$ must be 0. Thus, the matrix $A$ is null matrix.\\
	So the conclusion, if and only if matrix $A$ is 0, it's Frobenius norm is 0.\\
	\textbf{homogeneity}\\
	The Frobenius norm of $tA$ (where $t$ is a constant) is 
	\begin{equation}
	\lVert tA\rVert_F=\sqrt{\sum_{i=1}^m\sum_{j=1}^n(tA_{ij})^2}=\mid t\mid\sqrt{tr(A^TA)}=\mid t\mid\lVert A\rVert_F
	\end{equation}
	So it fulfill the property of homogeneity.\\
	\textbf{triangle inequality}
	\begin{equation}
	\lVert A+B\rVert_F=\sqrt{\sum_{i=1}^m\sum_{j=1}^n(A_{ij}+B_{ij})^2}
	\end{equation}
	Extract one arbitrary element for example, $\sqrt{(A_{ij}+B_{ij})^2}=\mid A_{ij}+B_{ij}\mid$, and it's not hard to get 
	\begin{equation}
	\mid A_{ij}+B_{ij}\mid \le \mid A_{ij}\mid +\mid B_{ij}\mid
	\end{equation}
	so we could get the conclusion 
	\begin{equation}
	\sqrt{\sum_{i=1}^m\sum_{j=1}^n(A_{ij}+B_{ij})^2} \le \sqrt{\sum_{i=1}^m\sum_{j=1}^n A_{ij}^2} + \sqrt{\sum_{i=1}^m\sum_{j=1}^n B_{ij}^2}
	\end{equation}
	\begin{equation}
	\lVert A+B\rVert_F\le \lVert A\rVert_F+\lVert B\rVert_F
	\end{equation}
	Therefore, Frobenius norm fulfill the property of triangle inequality as well.
	
	%%%%%%%%%%%%%%%%%%%%%%%%%%%%%%%%%%%%%%%%%%%%%%%%%%%%%%%%%%%%%%%%%%%%%%%%%%%%%%%%%%%%%%%%
	%%%%%%   question 4, sub question (b)
	%%%%%%%%%%%%%%%%%%%%%%%%%%%%%%%%%%%%%%%%%%%%%%%%%%%%%%%%%%%%%%%%%%%%%%%%%%%%%%%%%%%%%%%%
	\subsection*{(b)}
	According to the definition, $\lVert A^TA\rVert_F^2=\sum_{i=1}^n\sum_{j=1}^na_{ij}^2$.
	While the $ii$th element of $A^TA$ is
	
	\begin{equation}\label{aTa}
	\begin{split}
	(A^TA)_{ii}=&
	\left(  
	\left(  
	\begin{array}{cccc}
	a_{11} & a_{21} & \cdots & a_{n1}\\
	a_{12} & a_{22} & \cdots & a_{n2}\\
	\vdots \\
	a_{1n} & a_{2n} & \cdots & a_{nn}\\
	\end{array}
	\right)
	\left(  
	\begin{array}{cccc}
	a_{11} & a_{12} & \cdots & a_{1n}\\
	a_{21} & a_{22} & \cdots & a_{2n}\\
	\vdots \\
	a_{n1} & a_{n2} & \cdots & a_{nn}\\
	\end{array}
	\right)
	\right)_{ii} \\
	=\sum_{k=1}^n a^2_{ki}
	\end{split}
	\end{equation}
	Therefore, the trace of $A^TA$ is 
	\begin{equation}\label{trace_aTa}
	tr(A^TA) = \sum_{i=1}^n (A^TA)_{ii}=\sum_{i=1}^n\sum_{k=1}^n a^2_{ki}
	\end{equation}
	So we can say $\lVert A^TA\rVert_F^2=tr(A^TA)$. And then
	\begin{equation}\label{trAA_from}
	\nabla_A(\lVert A\rVert_F^2)=\nabla_A(tr(A^TA))
	\end{equation}
	then this question is the same as question 3(c), from equation and (\ref{aa_ii}) and (\ref{trAA_grad})
	we can get
	\begin{equation}\label{trAA_from_final}
	\nabla_A(\lVert A\rVert_F^2)=2A
	\end{equation}
	
	% --------------------------------------------------------------
	%     You don't have to mess with anything below this line.
	% --------------------------------------------------------------
	
\end{document}